Prove theorem about reading from file

examples/vipr/viprProgScript.sml
@@ -104,6 +104,65 @@ Proof
   \\ xsimpl
 QED
 
+Definition filename_ok_def:
+  filename_ok name ⇔
+    ¬MEM #"\^@" (explode name) ∧ strlen name < 256 * 256
+End
+
+Theorem main_spec_file:
+   hasFreeFD fs ∧ file_content fs (EL 1 cl) = SOME text ∧ 1 < LENGTH cl ∧
+   filename_ok (EL 1 cl)
+   ⇒
+   app (p:'ffi ffi_proj) main_v
+     [Conv NONE []]
+     (STDIO fs * COMMANDLINE cl)
+     (POSTv uv. &UNIT_TYPE () uv *
+                STDIO (add_stdout fs $
+                         run_vipr (lines_of (implode text))) *
+                COMMANDLINE cl)
+Proof
+  strip_tac
+  \\ xcf_with_def () main_v_def
+  \\ reverse $ xhandle ‘(POSTv uv. &UNIT_TYPE () uv *
+                STDIO (add_stdout fs $
+                         run_vipr (lines_of (implode text))) *
+                COMMANDLINE cl)’
+  >- xsimpl
+  \\ xlet_auto >- (xcon \\ xsimpl)
+  \\ reverse(Cases_on`wfcl cl`) >- (fs[COMMANDLINE_def] \\ xpull)
+  \\ fs[wfcl_def]
+  \\ xlet_auto >- xsimpl
+  \\ xlet_auto >- xsimpl
+  \\ assume_tac checker_step_v_thm
+  \\ assume_tac init_state_v_thm
+  \\ drule_then drule foldLines_SOME
+  \\ fs []
+  \\ disch_then $ drule_at $ Pos last \\ fs []
+  \\ rename [‘OPTION_TYPE STRING_TYPE (oHD (TL cl)) vvv’]
+  \\ ‘OPTION_TYPE FILENAME (SOME (EL 1 cl)) vvv’ by
+    (Cases_on ‘cl’ \\ fs [] \\ Cases_on ‘t’ \\ fs [std_preludeTheory.OPTION_TYPE_def]
+     \\ fs [FILENAME_def,filename_ok_def])
+  \\ disch_then drule
+  \\ disch_then $ qspec_then ‘p’ mp_tac
+  \\ strip_tac
+  \\ xlet ‘(POSTv retv.
+             STDIO fs * COMMANDLINE cl *
+             &OPTION_TYPE VIPRPROG_READER_STATE_TYPE
+               (SOME
+                  (foldl checker_step init_state (lines_of (implode text))))
+               retv)’
+  >- (xapp \\ xsimpl)
+  \\ qpat_x_assum ‘app _ _ _ _ _’ kall_tac
+  \\ xlet_auto >- xsimpl
+  \\ xlet_auto >- xsimpl
+  \\ xapp
+  \\ xsimpl
+  \\ pop_assum $ irule_at $ Pos hd
+  \\ fs [GSYM run_vipr_def]
+  \\ qexists_tac ‘fs’
+  \\ xsimpl
+QED
+
 Theorem vipr_stdin_whole_prog_spec:
    hasFreeFD fs ∧ stdin_content fs = SOME text ∧ LENGTH cl < 2 ⇒
    whole_prog_spec main_v cl fs NONE ((=) $ add_stdout (fastForwardFD fs 0) $
@@ -123,10 +182,33 @@ Proof
   \\ gvs [IO_fs_component_equality]
 QED
 
-val (sem_thm,prog_tm) = whole_prog_thm
-                          (get_ml_prog_state())
-                          "main"
-                          (UNDISCH vipr_stdin_whole_prog_spec)
+Theorem vipr_file_whole_prog_spec:
+   hasFreeFD fs ∧ file_content fs (EL 1 cl) = SOME text ∧ 1 < LENGTH cl ∧
+   filename_ok (EL 1 cl) ⇒
+   whole_prog_spec main_v cl fs NONE ((=) $ add_stdout fs $
+                                              run_vipr (lines_of (implode text)))
+Proof
+  rw[whole_prog_spec_def]
+  \\ irule_at Any app_wgframe
+  \\ irule_at Any main_spec_file
+  \\ fs []
+  \\ rpt $ first_assum $ irule_at Any
+  \\ xsimpl
+  \\ qexists_tac ‘(add_stdout fs
+               (run_vipr (lines_of (implode text))))’
+  \\ gvs [] \\ xsimpl
+  \\ gvs [GSYM add_stdo_with_numchars,with_same_numchars]
+QED
+
+val (stdin_thm,prog_tm) = whole_prog_thm
+                            (get_ml_prog_state())
+                            "main"
+                            (UNDISCH vipr_stdin_whole_prog_spec);
+
+val (file_thm,prog_tm) = whole_prog_thm
+                            (get_ml_prog_state())
+                            "main"
+                            (UNDISCH vipr_file_whole_prog_spec);
 
 Definition vipr_prog_def:
   vipr_prog = ^prog_tm
@@ -138,13 +220,25 @@ Proof
   fs []
 QED
 
-Theorem vipr_semantics =
-  sem_thm |> REWRITE_RULE[GSYM vipr_prog_def]
+Theorem vipr_stdin_semantics =
+  stdin_thm
+  |> REWRITE_RULE[GSYM vipr_prog_def]
   |> DISCH_ALL
   |> SIMP_RULE(srw_ss())[GSYM CONJ_ASSOC,AND_IMP_INTRO]
   |> MATCH_MP clean_up
   |> Q.SPEC ‘stdin_content fs = SOME text ∧ LENGTH cl < 2 ∧ wfcl cl ∧
              wfFS fs ∧ STD_streams fs ∧ hasFreeFD fs’
+  |> CONV_RULE ((RATOR_CONV o RAND_CONV) (SIMP_CONV (srw_ss()) []))
+  |> (fn th => MATCH_MP th TRUTH);
+
+Theorem vipr_file_semantics =
+  file_thm
+  |> REWRITE_RULE[GSYM vipr_prog_def]
+  |> DISCH_ALL
+  |> SIMP_RULE(srw_ss())[GSYM CONJ_ASSOC,AND_IMP_INTRO]
+  |> MATCH_MP clean_up
+  |> Q.SPEC ‘hasFreeFD fs ∧ file_content fs (EL 1 cl) = SOME text ∧ 1 < LENGTH cl ∧
+             filename_ok (EL 1 cl) ∧ wfcl cl ∧ wfFS fs ∧ STD_streams fs’
   |> CONV_RULE ((RATOR_CONV o RAND_CONV) (SIMP_CONV (srw_ss()) []))
   |> (fn th => MATCH_MP th TRUTH);
 
